core/Peo.v
@@ -1,5 +1,3 @@
-From Ssara.Core Require Import RegClass.
-From Ssara.Core Require Import RegSet.
 From Ssara.Core Require Import InterfGraph.
 From Ssara.Core Require Import Dict.
 From Ssara.Core Require Import Utils.
@@ -7,28 +5,28 @@ From Stdlib Require Import ZArith.
 From Stdlib Require Import Lists.List.
 From Stdlib Require Import Bool.
 
-From Ssara.Core Require Import RegVregInstance.
-Existing Instance reg_vreg_instance.
+From Ssara.Core Require Import IRVregModule.
+Import IRVreg.
 
 (* Check whether regs are neighbors of r *)
-Definition are_neighbors (g : ig) (r : reg) (regs : list reg) : bool :=
-  regs_mem r (dict_keys g) &&
-  conjunction (fun r' => (r =? r') || regs_mem r' (dict_map g r)) regs
+Definition are_neighbors (g : InterfGraph.dict) (r : reg) (regs : list reg) : bool :=
+  regs_mem r (InterfGraph.keys g) &&
+  conjunction (fun r' => (r =? r') || regs_mem r' (InterfGraph.get g r)) regs
 .
 
 (* Check whether the neighbors of r are a clique *)
-Definition is_simplicial (g : ig) (r : reg) : bool :=
-  let regs := dict_map g r in
-  regs_mem r (dict_keys g) &&
+Definition is_simplicial (g : InterfGraph.dict) (r : reg) : bool :=
+  let regs := InterfGraph.get g r in
+  regs_mem r (InterfGraph.keys g) &&
   conjunction (fun r' => are_neighbors g r' regs) regs
 .
 
-Definition find_next (g : ig) : option reg :=
-  find (is_simplicial g) (dict_keys g)
+Definition find_next (g : InterfGraph.dict) : option reg :=
+  find (is_simplicial g) (InterfGraph.keys g)
 .
 
 Lemma find_next_in :
-  forall (g : ig) (n : reg), find_next g = Some n -> In n (dict_keys g)
+  forall (g : InterfGraph.dict) (n : reg), find_next g = Some n -> In n (InterfGraph.keys g)
 .
 Proof.
   intros g n. unfold find_next. apply find_some.
@@ -37,7 +35,7 @@ Qed.
 From Stdlib Require Import FunInd.
 From Stdlib Require Import Recdef.
 
-Function eliminate (g : ig) {measure dict_size g} : list vreg :=
+Function eliminate (g : InterfGraph.dict) {measure InterfGraph.size g} : list vreg :=
   match find_next g with
   | Some next =>
     let g := ig_remove_node g next in
