core/IRVregModule.v
@@ -1,0 +1,13 @@
+From Stdlib Require Import PeanoNat.
+From Stdlib Require Import ListSet.
+From Ssara.Core Require Import IR.
+
+Definition vreg : Set := nat.
+
+Module IRVregParams <: IR_PARAMS.
+  Definition reg := vreg.
+  Definition reg_eqb := Nat.eqb.
+  Definition reg_eq_dec := Nat.eq_dec.
+End IRVregParams.
+
+Module IRVreg := MakeIR IRVregParams.
