core/RegClass.v
@@ -1,5 +1,0 @@
-Class RegClass := {
-  reg : Set;
-  reg_eqb : reg -> reg -> bool;
-  reg_eq_dec : forall r r' : reg, {r = r'} + {r <> r'};
-}.
